ocaml/grammar.ml
@@ -9,19 +9,20 @@ top_item ::= fn_def | struct_def | trait_def | impl_def
 
 ## top-level items
 ```
-fn_def ::= "fn" ID opt_lifetime_params "(" params ")" "->" ty opt_where_outlives "{" block "}"
+fn_def ::= "fn" ID opt_generic_params "(" params ")" "->" ty opt_fn_where_clause "{" block "}"
 struct_def ::= "struct" ID opt_generic_params opt_trait_bounds "{" struct_field ("," struct_field)* "}"
 trait_def ::= "trait" ID opt_generic_params opt_trait_bounds ";"
 impl_def ::= "impl" opt_generic_params ID opt_type_args "for" ty ";"
 struct_field ::= opt_mut ID ":" ty
 trait_bound ::= ID ":" trait_ref ("+" trait_ref)*
 trait_ref ::= ID opt_type_args
+opt_fn_where_clause ::= ""
+                      | "where" fn_where_item ("," fn_where_item)*
+fn_where_item ::= trait_bound | outlives_constraint
 ```
 
 ## generic params and bounds
 ```
-opt_lifetime_params ::= ""
-                      | "<" LIFETIME ("," LIFETIME)* ">"
 opt_generic_params ::= ""
                      | "<" generic_param ("," generic_param)* ">"
 generic_param ::= LIFETIME | ID
